partial implementation of dijkstra

Graphs/Graph.lean
@@ -68,6 +68,13 @@ def K1 := Graph.mk [1] [] (by simp)
 def K2 := Graph.mk [1, 2] [Edge.mk 1 1 2] (by simp)
 def K3 := Graph.mk [1, 2, 3] [Edge.mk 1 1 2, Edge.mk 2 2 3, Edge.mk 3 3 1] (by simp)
 
+def KEdges (n : Nat) (xs : List Nat) : List Edge :=
+    match xs with
+    | [] => []
+    | y::ys => List.map (λ x => Edge.mk (x - y + n) y x) ys ++ KEdges (n + ys.length) ys
+
+def K (n : Nat) := Graph.mk ((List.iota n).reverse) (KEdges 0 (List.iota n).reverse)
+
 def K0 := instInhabitedGraph.default
 
 #eval K0.isNull
@@ -82,10 +89,164 @@ def K0 := instInhabitedGraph.default
 
 #eval K1.adjacent ((K1.N.get? 0).get (by simp; decide)) ((K3.N.get? 2).get (by simp; decide))
 
+#eval K 7 (by simp; decide)
+
 def e1 := (K3.E.get? 1).get (by decide)
 def e2 := (K3.E.get? 2).get (by decide)
 
 #eval Graph.parallel K3 e1 e2
 
+
+
+def L (n : Node) (l : List (Node × (Node × Int))) : Int :=
+match l.filter (λ (x,_) => x == n) with
+| [] => 0
+| x::_ => x.2.2
+
+def LPair (n : Node) (l : List (Node × (Node × Int))) : (Node × Node × Int) :=
+match l.filter (λ (x,_) => x == n) with
+| [] => (0,0,0)
+| x::_ => (n, x.2.1, x.2.2)
+
+def newL (n : Node) (v : Nat) (l : List (Node × (Node × Int))) : List (Node × (Node × Int)) :=
+match l with
+| [] => l
+| x::xs => if n == x.1 then (n,(x.2.1, v))::xs else x::(newL n v xs)
+
+#eval newL 2 4 [(2,(0,1)), (3,(0,1))]
+#eval L 2  <| newL 2 4 [(2,(0,1)), (3,(0,1))]
+#eval LPair 2 [(2, 0, 4), (3, 0, 1)]
+
+structure WGraph where
+  N : List Node
+  E : List Edge
+  W : List (Edge × Nat)
+  ok : (∀ e, e ∈ E → (e.i ∈ N ∧ e.j ∈ N))
+       ∧ (∀ e, e ∈ E → (∃ w, w ∈ W ∧ e = w.1))
+       ∧ unique N
+       ∧ unique E
+       ∧ unique W
+
+instance : Inhabited WGraph where
+  default := WGraph.mk [] [] [] (by simp [unique])
+
+instance : Repr WGraph where
+  reprPrec g _ :=
+    let formatNode := fun n => (f!"v{n}")
+    let formatWeights := fun w => (f!"({repr w.1}, w:{w.2})")
+    f!"(N={List.map formatNode g.N}, E={repr g.E} W={List.map formatWeights g.W})"
+
+#eval WGraph.mk [1,2,3] [Edge.mk 1 1 2, Edge.mk 2 2 3] [((Edge.mk 1 1 2), 3), ((Edge.mk 2 2 3), 1)] (by simp)
+
+
+def findMinL  (v : (Node × Int)) (l : List (Node × (Node × Int))) : (Node × Int) :=
+match l with
+| [] => v
+| x::xs => if (x.2.2 < v.2 ∧ x.2.2 != -1) ∨ v.2 == -1 then findMinL x.2 xs else findMinL v xs
+
+def MinLNode (p : Node × (Node × Int)) (l : List (Node × (Node × Int))) : Node :=
+  match l with
+  | [] => p.1
+  | x::xs => if p.2.2 == x.2.2 then MinLNode (x.1, p.2) [] else MinLNode p xs
+  termination_by l.length
+
+#eval (fun x => MinLNode (0,x) [(1,0,3), (2,0,2), (3,0,1), (4,0,3)]) <| findMinL (0,-1) [(1,0,2), (2,0,2), (3,0,1), (4,0,3)]
+
+def new_Ls (ns : List Node) (v : Int) : List (Node × (Node × Int)) :=
+ns.map (fun x => (x,(0, v)))
+
+#eval newL 1 0 <| new_Ls (K 3 (by simp; decide)).N (-1)
+
+def Node.adjacent (es : List Edge) (n m : Node) := ∃ e, e ∈ es ∧ e.incident n ∧ e.incident m ∧ n ≠ m
+
+instance : Decidable (Node.adjacent es n m) := by
+  simp [Node.adjacent, Edge.incident]; exact List.decidableBEx _ es
+
+
+def filterAdj (n : Node) (g : List Node) (es : List Edge) : List Node :=
+  g.filter (Node.adjacent es n)
+
+#eval filterAdj 1 (K 4 (by simp; decide)).N (K 4 (by simp; decide)).E
+#eval (K 4 (by simp; decide)).adjacent 1 1
+
+def findWeight (v n : Node) (ws : List (Edge × Int)) : Int :=
+  match ws with
+  | [] => 0
+  | x::xs =>
+    if (Edge.incident x.1 v) ∧ (Edge.incident x.1 n) then x.2
+    else findWeight v n xs
+
+#eval findWeight 1 2 [(Edge.mk 1 2 3, 3), (Edge.mk 1 1 2, 4)]
+
+def updateLs (v n : Node) (l : List (Node × (Node × Int))) (ws : List (Edge × Int))
+    : List (Node × (Node × Int)) :=
+    let n_l := L n l
+    let vn_w := findWeight v n ws
+    let minimum := if n_l == -1 then (L v l) + vn_w else min n_l ((L v l) + vn_w)
+    if minimum == n_l then l else help n l minimum where
+    help (n : Node) (l : List (Node × (Node × Int))) (label : Int) : List (Node × (Node × Int)) :=
+    match l with
+    | [] => []
+    | x::xs => if x.1 == n then (n,(v,label))::xs else x::(help n xs label)
+
+def UpdateLsMap (v : Node) (ns : List Node) (l : List (Node × (Node × Int)))  (ws : List (Edge × Int))
+  : List (Node × (Node × Int)) :=
+  List.foldr (fun x y => updateLs v x y ws) l ns
+
+#eval UpdateLsMap 1 [2, 3] [(1, 0, 2), (2, 0, 4), (3, 0, 4)] [(Edge.mk 1 1 3, 1), (Edge.mk 1 1 2, 1)]
+#eval UpdateLsMap 1 [2, 3] [(1, 0, 2), (2, 0, 4), (3, 0, 4)] [(Edge.mk 1 1 3, 3), (Edge.mk 1 1 2, 4)]
+
+def isinGraph (n : Node) (ns : List Node) : Bool :=
+  if (ns.filter (· == n)).length >= 1 then true else false
+
+#eval isinGraph 1 [2,3]
+
+def t1 : (new_Ls [a] (-1))++(new_Ls as (-1)) = new_Ls (a::as) (-1) := by
+      induction as with
+      | nil => rfl
+      | cons b bs _ =>
+        rfl
+
+example : ∀ v, v ∈ T → (fun x => MinLNode (0,x) (UpdateLsMap v (filterAdj v T es) (new_Ls T (-1)) ws)) (findMinL (0,-1)  (UpdateLsMap v (filterAdj v T es) (new_Ls T (-1)) ws)) ∈ T := by
+  simp
+  induction T with
+  | nil => simp
+  | cons a as ih =>
+    intro v
+    intro h
+    rw [←t1]
+    simp
+    sorry
+
+-- definition still partial
+partial def dijkstra (a z : Node) (G : Graph) (W : List (Edge × Int)) : List (Node × (Node × Int)) :=
+  let labels := newL a 0 <|new_Ls G.N (-1)
+  let T := G.N
+  if T.length = 0 then [(0,(0,0))] else
+    help  z T labels T G.E W [] where
+    help (z : Node) (t : List Node) (ls : List (Node × (Node × Int)))
+      (N : List Node) (es : List Edge) (ws : List (Edge × Int)) (f : List (Node × (Node × Int)))
+      : List (Node × Node × Int) :=
+      if (isinGraph z t) then
+        let v := (fun x => MinLNode (0,x) ls) <| findMinL (0,-1) ls
+        let v_l := (LPair v ls)
+        let ads := filterAdj v N es
+        let new_lbs := List.filter (fun x => x.1 != v) (UpdateLsMap v ads ls ws)
+        let T := t.filter (fun x => x != v)
+        help z T new_lbs N es ws (f++[v_l])
+      else f
+
+def SimpleW (E : List Edge) : List (Edge × Int) :=
+ match E with
+ | [] => []
+ | x::xs => (x,1)::(SimpleW xs)
+
+def ChangeW (v : Int) (e : Edge) (W : List (Edge × Int)) : List (Edge × Int) :=
+match W with
+| [] => []
+| x::xs => if x.1 == e then (x.1,v)::xs else x::(ChangeW v e xs)
+
+#eval ChangeW 3 (Edge.mk 1 1 2) <| SimpleW (K 4 (by simp; decide)).E
+#eval dijkstra 1 3 (K 3 (by simp; decide)) [(Edge.mk 1 1 3, 5), (Edge.mk 2 1 2, 1), (Edge.mk 3 3 2, 1)]
 
 end GraphTheory
